theories/cancellation/CancelGetTid.v
@@ -11,21 +11,33 @@ Local Ltac sir :=
 Local Ltac snr := norm_r; rewrite !list_insert_insert ?bind_ret_l.
 
 Lemma cancel_gettid `{_crisG: !crisG Γ Σ α β τ _S _I, _concG: !concG} md sp 
-  (X: Type) (PQ: X → (Any.t → iProp Σ) * (Any.t → iProp Σ)) N mm stid :
-  CANCEL_GOAL md sp PQ N mm (HoareGetTidE false stid) (HoareGetTidE true stid).
+  (X: Type) (PQ: X → (Any.t → iProp Σ) * (Any.t → iProp Σ)) mm :
+  CANCEL_GOAL md sp PQ mm (HoareGetTidE false) (HoareGetTidE true).
 Proof.
   r; i. subst.
 
   iter_l. rewrite x0 /=. step_l. norm_l.
-  iter_r. rewrite x1 /=. step_r. norm_r. rewrite !bind_ret_l.
+  iter_r. rewrite x1 /=. step_r. i. norm_r. rewrite !bind_ret_l.
 
-  sil. step_l. snl. rewrite Any.pair_split /= !bind_ret_l Any.upcast_downcast /= !bind_ret_l.
-  sir. step_r. i. step_r. snr.
+  sil. step_l. snl.
+  (* rewrite Any.pair_split /= !bind_ret_l Any.upcast_downcast /= !bind_ret_l. *)
+  (* sir. *)
+  step_r. i. norm_r.
+  (* snr. *)
   (* sir. step_r. i. *)
   (* sir. step_r. snr. rewrite Any.pair_split /= !bind_ret_l Any.upcast_downcast /= !bind_ret_l. *)
   (* sir. step_r. i. step_r. snr. *)
+  (* sir. step_r. i. step_r. snr. *)
+  sir. step_r. snr.
+  (* sir. step_r. snr. *)
+  (* rewrite Any.pair_split /= !bind_ret_l.
+  sir. step_r. snr.
+  sir. step_r. snr.
+  sir. step_r. snr. *)
+  sir. step_r. snr. rewrite Any.pair_split /= !bind_ret_l Any.upcast_downcast /= !bind_ret_l.
   sir. step_r. i. step_r. snr.
-  sir. step_r. snr. rewrite Any.pair_split /= !bind_ret_l.
+  sir. step_r. i. step_r. snr.
+  sir. step_r. snr. hss. ired.
   sir. step_r. snr.
   sir. step_r. snr.
   sir. step_r. snr.
@@ -36,10 +48,10 @@ Proof.
   { des; split; eauto.
     { eapply Own_wand_valid with (a1 := r_s); eauto. rewrite RS.
       iIntros ">[_ [$ _]]"; eauto. }
-    rewrite x4. iIntros ">[$ $]". iPureIntro. sym.
+    rewrite x5. iIntros ">[$ $]". iPureIntro. sym.
     eapply Own_pure_soundness with (a:=r_s); eauto.
     iIntros "S". iPoseProof (RS with "S") as ">[_ [T [TA _]]]".
-    iPoseProof (x4 with "T") as ">[T _]".
+    iPoseProof (x5 with "T") as ">[T _]".
     iApply (TidToken_agree with "[T]"); iFrame.
   }
   step_r. snr.
