theories/cancellation/CancelYield.v
@@ -19,21 +19,24 @@ Local Ltac sir :=
 Local Ltac snr := norm_r; rewrite !list_insert_insert ?bind_ret_l.
 
 Lemma cancel_yield `{_crisG: !crisG Γ Σ α β τ _S _I, _concG: !concG} md sp
-  (X: Type) (PQ: X → (Any.t → iProp Σ) * (Any.t → iProp Σ)) sN tN mm stid ttid ntid :
-  CANCEL_GOAL md sp PQ tN mm (HoareYieldE false sN stid ntid) (HoareYieldE true tN ttid ntid).
+  (X: Type) (PQ: X → (Any.t → iProp Σ) * (Any.t → iProp Σ)) mm ntid :
+  CANCEL_GOAL md sp PQ mm (HoareYieldE false ntid) (HoareYieldE true ntid).
 Proof.
   r; i. subst.
   iter_l; iter_r. rewrite x0 x1 /=.
   step_l. norm_l. rewrite !bind_ret_l.
-  step_r. i. ired. rewrite Any.pair_split /= bind_ret_l Any.upcast_downcast /= bind_ret_l. norm_r.
+  step_r. intros ttid. ired.
+  
   (* step_r. norm_r. rewrite !bind_ret_l. *)
 
   (* sir. step_r. snr. sir. step_r. snr. *)
   (* rewrite Any.pair_split /= bind_ret_l Any.upcast_downcast /= bind_ret_l. *)
-  norm_r.
-  sir. step_r. i. step_r. snr. sir. step_r. i. step_r. snr.
-  sir. step_r. snr. rewrite Any.pair_split /= bind_ret_l.
-  sir. step_r. snr. sir. step_r. snr. sir. step_r. snr.
+  norm_r. step_r. norm_r. sir. step_r. snr. sir. step_r. snr.
+  rewrite Any.pair_split /= bind_ret_l Any.upcast_downcast /= bind_ret_l.
+  (* step_r. snr. *)
+  sir. step_r. i. step_r. snr.
+  sir. step_r. i. step_r. snr. sir. step_r. snr. rewrite Any.pair_split /=. sir. step_r. snr.
+  sir. step_r. snr. sir. step_r. snr.
   
   des.
   assert (EQ: ttid = cid).
@@ -43,26 +46,27 @@ Proof.
     iApply (TidToken_agree with "T"); iFrame. }
   subst.
 
-  assert (RS0: Own r_s ⊢
-                 |==> (([∗ list] i ∈ rs_diff, Own i) ∗ TIDAUTH ntid ∗ YIELDAUTH (length rs_diff)) ∗
-                 ((TID ntid ∗ YIELD ntid ∗ winv (↑tN, ↑tN)) ∗ Own x)).
-  { rewrite RS x4. iIntros ">[$ [>[[T [$ $]] $] [TA $]]]".
-  iApply (TidToken_upd with "[TA T]"); iFrame. }
-  hexploit (Own_bupd_split); eauto.
-  intros [r_t1 [r_t2 [Hr_t1 [Hr_t2 Hr_t3]]]].
-
-  assert (TVALID: ✓ r_t2).
-  { eapply Own_wand_valid with (a1:=r_s); eauto.
-    rewrite Hr_t1. iIntros ">[_ $]"; eauto. }
-
   destruct (decide (ntid < length rs_diff)); cycle 1.
   {
     iter_l. destruct (<[cid:=_]> srcs !! ntid) eqn:FIND.
     { eapply lookup_lt_Some in FIND. rewrite length_insert in FIND. nia. }
     { step_l. rewrite /triggerUB. step_l. i; ss. }
   }
+  
+  assert (RS0: Own r_s ⊢
+        |==> (([∗ list] i ∈ rs_diff, Own i) ∗ TIDAUTH ntid ∗ YIELDAUTH (length rs_diff)) ∗
+        ((TID ntid ∗ YIELD ntid ∗ winv (⊤, ⊤)) ∗ Own x)).
+  { rewrite RS x4. iIntros ">[$ [>[[T [$ $]] $] [TA $]]]".
+    iApply (TidToken_upd with "[TA T]"); iFrame. }
+  hexploit (Own_bupd_split); eauto.
+  intros [r_t1 [r_t2 [Hr_t1 [Hr_t2 Hr_t3]]]].
+
+  assert (TVALID: ✓ r_t2).
+  { eapply Own_wand_valid with (a1:=r_s); eauto.
+    rewrite Hr_t1. iIntros ">[_ $]"; eauto. }
   destruct (decide (ntid = cid)); subst.
   {
+    
     sil. step_l. snl. sir. step_r. snr. sir. step_r. snr.
     rewrite Any.pair_split /= bind_ret_l Any.upcast_downcast /= bind_ret_l.
     sir. step_r. exists r_t2. step_r. snr. sir. step_r. 
@@ -70,33 +74,51 @@ Proof.
     { des; split; eauto. rewrite Hr_t3. eapply bupd_intro. }
     step_r. snr. sir. step_r. snr. rewrite Any.pair_split /= bind_ret_l.
     sir. step_r. snr. sir. step_r. snr.
-
     eapply KEY with (r_diff:=ε); eauto.
     { rewrite length_insert list_insert_id //.
       iIntros "S". iPoseProof (Hr_t1 with "S") as ">[S $]"; iStopProof.
       rewrite Hr_t2. eapply bupd_intro. }
     { eapply thread_rel_body; eauto. eapply KTR. }
   }
-  { do 2 dup l. rename l into SRC, l0 into TGT, l1 into RES.
+  {
+  revert n; clear_until l; intros n.
+  assert (Hntid : is_Some (rs_diff !! ntid)).
+  { rewrite lookup_lt_is_Some //. }
+  destruct Hntid as [rsntid Hntid].
+  assert (RS0: Own r_s ⊢
+                 |==> (([∗ list] i ∈ <[ntid:=ε]> rs_diff, Own i) ∗ TIDAUTH ntid ∗ YIELDAUTH (length rs_diff)) ∗
+                 ((TID ntid ∗ YIELD ntid ∗ winv (⊤, ⊤)) ∗ Own (rsntid) ∗ Own x)).
+  { rewrite RS x4. iIntros ">[A [>[[T [$ $]] $] [TA $]]]".
+    iPoseProof (TidToken_upd with "[TA T]") as "> [$ $]"; iFrame.
+    iPoseProof (big_sepL_insert_acc with "A") as "[$ A]"; auto using Hntid.
+    iApply "A"; iApply Own_unit.
+  }
+  hexploit (Own_bupd_split); eauto.
+  intros [r_t1 [r_t2 [Hr_t1 [Hr_t2 Hr_t3]]]].
+
+  assert (TVALID: ✓ r_t2).
+  { eapply Own_wand_valid with (a1:=r_s); eauto.
+    rewrite Hr_t1. iIntros ">[_ $]"; eauto. }
+
+     do 2 dup l. rename l into SRC, l0 into TGT, l1 into RES.
     rewrite EQLEN2 in SRC. rewrite EQLEN2 EQLEN in TGT.
     dup SRC; dup TGT; dup RES.
     eapply list_lookup_exists in SRC, TGT, RES; des.
     hexploit REL; eauto; intros RELTID. inv RELTID.
     { (* first execution *)
       iter_l; iter_r. rewrite !list_lookup_insert_ne // SRC TGT /=.
-      step_l. norm_l. step_r. exists (tN, ntid). step_r. norm_r.
-      sil. step_l. snl.
-      sir. step_r. snr. sir. step_r. exists x8. step_r. snr.
+      step_l. norm_l. step_r. exists x8. step_r. norm_r.
       sir. step_r. snr. sir. step_r. exists varg. step_r. snr.
       sir. step_r. snr. sir. step_r. snr.
       rewrite Any.pair_split /= bind_ret_l Any.upcast_downcast /= bind_ret_l.
       sir. step_r. exists r_t2. step_r. snr.
       sir. step_r. unshelve eexists.
-      { split; eauto. rewrite Hr_t3. iIntros "[$ $]"; eauto. }
+      { split; eauto. rewrite Hr_t3 H4. iIntros "[[? [? ?]] [> A $]]"; iApply ("A" with "[$] [$] [$]"). }
+      s. ired.
       step_r. snr.
       sir. step_r. snr. rewrite Any.pair_split /= bind_ret_l.
       sir. step_r. snr. sir. step_r. snr.
-      sir. step_r. snr. rewrite Any.pair_split /= bind_ret_l Any.upcast_downcast /= bind_ret_l.
+      (* sir. step_r. snr. rewrite Any.pair_split /= bind_ret_l Any.upcast_downcast /= bind_ret_l.
       sir. step_r. exists (x7 ⋅ r_t2). step_r. snr.
       sir. step_r. unshelve eexists.
       { split; eauto.
@@ -108,7 +130,8 @@ Proof.
       }
       step_r. snr. sir. step_r. snr. rewrite Any.pair_split /= bind_ret_l.
       sir. step_r. snr. sir. step_r. snr.
-      rewrite /ModTr.trans in TGT.
+      rewrite /ModTr.trans in TGT. *)
+      sil. step_l. snl.
 
       gstep. econs. econs; try exact smj_lt_mid_top.
       gbase. eapply CIH with (rs_diff:=<[ntid:=ε]>rs_diff); eauto.
@@ -137,10 +160,12 @@ Proof.
         }
       }
       {
-        rewrite Hr_t1 Hr_t2 Own_op -!assoc (assoc _ _ (Own x7)) length_insert.
-        iIntros ">(D & $ & $ & $)". iModIntro.
+        rewrite Hr_t1 Hr_t2 length_insert.
+        (* Own_op -!assoc (assoc _ _ (Own x7)) length_insert. *)
+        iIntros ">[[$ $] $] //".
+        (* iModIntro.
         iPoseProof (big_sepL_insert_acc with "D") as "[$ D]"; [eapply RES|].
-        iApply "D". iApply Own_unit.
+        iApply "D". iApply Own_unit. *)
       }
     }
     { (* middle of execution *)
@@ -150,7 +175,7 @@ Proof.
       rewrite Any.pair_split /= bind_ret_l Any.upcast_downcast /= bind_ret_l.
       sir. step_r. exists r_t2. step_r. snr.
       sir. step_r. unshelve eexists.
-      { split; eauto. rewrite Hr_t3. eapply bupd_intro. }
+      { split; eauto. rewrite Hr_t3. iIntros "[$ [? $]] //". }
       step_r. snr.
       sir. step_r. snr. rewrite Any.pair_split /= bind_ret_l.
       sir. step_r. snr. sir. step_r. snr.
@@ -183,9 +208,10 @@ Proof.
       }
       {
         rewrite Hr_t1 Hr_t2 -!assoc length_insert.
-        iIntros ">(D & $ & $ & $)". iModIntro.
+        iIntros ">($ & $ & $ & $) //".
+        (* iModIntro.
         iPoseProof (big_sepL_insert_acc with "D") as "[_ D]"; [eapply RES|].
-        iApply "D". iApply Own_unit.
+        iApply "D". iApply Own_unit. *)
       }
     }
   }
